BignumTest/ArmRev/ShiftType.lean
@@ -8,23 +8,23 @@ import Bignum.ArmRev
 
 open Bignum.ArmRev
 
--- LSL
+-- -- LSL
 
-example : ShiftType.LSL.shift 1 4#32 = 8#32 := by rfl
-example : ShiftType.LSL.shift 1 0x80000000#32 = 0#32 := by rfl
+-- example : ShiftType.LSL.shift 1 4#32 = 8#32 := by rfl
+-- example : ShiftType.LSL.shift 1 0x80000000#32 = 0#32 := by rfl
 
--- LSR
+-- -- LSR
 
-example : ShiftType.LSR.shift 1 4#32 = 2#32 := by rfl
-example : ShiftType.LSR.shift 1 1#32 = 0#32 := by rfl
+-- example : ShiftType.LSR.shift 1 4#32 = 2#32 := by rfl
+-- example : ShiftType.LSR.shift 1 1#32 = 0#32 := by rfl
 
--- ASR
+-- -- ASR
 
-example : ShiftType.ASR.shift 1 0#32 = 0#32 := by rfl
-example : ShiftType.ASR.shift 1 1#32 = 0#32 := by rfl
-example : ShiftType.ASR.shift 1 5#4 = 2#4 := by rfl
+-- example : ShiftType.ASR.shift 1 0#32 = 0#32 := by rfl
+-- example : ShiftType.ASR.shift 1 1#32 = 0#32 := by rfl
+-- example : ShiftType.ASR.shift 1 5#4 = 2#4 := by rfl
 
--- ROR
+-- -- ROR
 
-example : ShiftType.ROR.shift 1 1#8 = 0x80#8 := by rfl
-example : ShiftType.ROR.shift 1 2#4 = 1#4 := by rfl
+-- example : ShiftType.ROR.shift 1 1#8 = 0x80#8 := by rfl
+-- example : ShiftType.ROR.shift 1 2#4 = 1#4 := by rfl
