BignumTest/BitVec.lean
@@ -1,0 +1,12 @@
+/-
+Copyright (c) 2026 Guilherme Lima. All rights reserved.
+Released under Apache 2.0 license as described in the file LICENSE.
+Author: Guilherme Lima
+-/
+
+import Bignum.BitVec
+
+open BitVec
+
+example : setLsb (0b0000#8) 3 true == 8#8 := by rfl
+example : setLsb (0b1010#8) 1 false == 8#8 := by rfl
